proof/invariant-abstract/RISCV64/ArchVSpaceEntries_AI.thy
@@ -295,7 +295,7 @@ begin
 
 crunches invoke_sched_context, invoke_sched_control_configure_flags
   for valid_vspace_objs'[wp]: "valid_vspace_objs'"
-  (ignore: update_sk_obj_ref wp: crunch_wps)
+  (ignore: update_sk_obj_ref wp: crunch_wps hoare_vcg_all_lift simp: crunch_simps)
 
 end
 
